refinements/DropEpochRedir.v
@@ -1,0 +1,204 @@
+Require Import Kami.
+Require Import Lib.CommonTactics Lib.Indexer Lib.VectorFacts.
+Require Import Kami.Decomposition Kami.ModuleBoundEx.
+Require Import Ex.MemTypes Ex.OneEltFifo.
+Require Import Proc.AbstractIsa Proc.Fetch Proc.Decode Proc.RegRead Proc.Execute
+        Proc.InOrderEightStage.
+Require Import DropBranchPredictors Fidre.
+
+Set Implicit Arguments.
+Open Scope string.
+
+Section Processor.
+  Variables addrSize dataBytes rfIdx: nat.
+
+  Variable decodeInst: DecodeT dataBytes rfIdx.
+  Variable execInst: ExecT addrSize dataBytes rfIdx.
+
+  (** Fetch related *)
+  Definition fetchNondet := fetchNondet addrSize dataBytes.
+  Definition fetchNondetNR := fetchNondetNR addrSize dataBytes f2iName.
+  Definition decRedir := decRedir addrSize.
+  Definition exeRedir := exeRedir addrSize.
+  Definition f2i := f2i addrSize dataBytes.
+
+  (** IMem related *)
+  Definition iMem := iMem addrSize dataBytes.
+  Definition i2d := i2d addrSize dataBytes.
+
+  (** Decode related *)
+  Definition decodeNondet := decodeNondet addrSize decodeInst.
+  Definition decodeNondetNR := decodeNondetNR addrSize i2dName d2rName decodeInst.
+  Definition d2r := d2r addrSize dataBytes rfIdx.
+
+  (** RegRead related *)
+  Definition regRead := regRead addrSize dataBytes rfIdx.
+  Definition rf := rf dataBytes rfIdx.
+  Definition bypass := bypass dataBytes rfIdx.
+  Definition r2e := r2e addrSize dataBytes rfIdx.
+
+  (** Execute related *)
+  Definition executeNondet := executeNondet execInst.
+  Definition executeNondetNR := executeNondetNR r2eName e2mName execInst.
+  Definition e2m := e2m addrSize dataBytes rfIdx.
+
+  (** Mem related *)
+  Definition mem := mem addrSize dataBytes rfIdx.
+  Definition m2d := m2d addrSize dataBytes rfIdx.
+
+  (** DMem related *)
+  Definition dMem := dMem addrSize dataBytes rfIdx.
+  Definition d2w := d2w addrSize dataBytes rfIdx.
+
+  (** Writeback related *)
+  Definition writeback := writeback addrSize dataBytes rfIdx.
+
+  Definition fidreComb := fidreComb decodeInst execInst.
+  
+  Definition fidreNR :=
+    (fetchNondetNR ++ f2i
+                   ++ iMem ++ i2d
+                   ++ decodeNondetNR ++ d2r
+                   ++ regRead ++ r2e
+                   ++ executeNondetNR)%kami.
+
+  Section RefinementNR.
+
+    Definition F2I := F2I addrSize dataBytes.
+    Definition I2D := I2D addrSize dataBytes.
+    Definition D2R := D2R addrSize dataBytes rfIdx.
+    Definition R2E := R2E addrSize dataBytes rfIdx.
+
+    Fixpoint getArchPcF2I (decEpoch exeEpoch: bool) (f2i: list (type (Struct F2I)))
+      : option (fullType type (SyntaxKind (Bit addrSize))) :=
+      match f2i with
+      | nil => None
+      | e :: f2i' =>
+        if (eqb (e Fin.F1 (Fin.FS (Fin.FS Fin.F1))) decEpoch &&
+                eqb (e Fin.F1 (Fin.FS (Fin.FS (Fin.FS Fin.F1)))) exeEpoch)
+        then Some (e Fin.F1 Fin.F1)
+        else getArchPcF2I decEpoch exeEpoch f2i'
+      end.
+
+    Fixpoint getArchPcI2D (decEpoch exeEpoch: bool) (i2d: list (type (Struct I2D)))
+      : option (fullType type (SyntaxKind (Bit addrSize))) :=
+      match i2d with
+      | nil => None
+      | e :: i2d' =>
+        if (eqb (e Fin.F1 (Fin.FS (Fin.FS Fin.F1))) decEpoch &&
+                eqb (e Fin.F1 (Fin.FS (Fin.FS (Fin.FS Fin.F1)))) exeEpoch)
+        then Some (e Fin.F1 Fin.F1)
+        else getArchPcI2D decEpoch exeEpoch i2d'
+      end.
+
+    Fixpoint getArchPcD2R (exeEpoch: bool) (d2r: list (type (Struct D2R)))
+      : option (fullType type (SyntaxKind (Bit addrSize))) :=
+      match d2r with
+      | nil => None
+      | e :: d2r' =>
+        if (eqb (e (Fin.FS (Fin.FS (Fin.FS Fin.F1)))) exeEpoch)
+        then Some (e Fin.F1)
+        else getArchPcD2R exeEpoch d2r'
+      end.
+
+    Fixpoint getArchPcR2E (exeEpoch: bool) (r2e: list (type (Struct R2E)))
+      : option (fullType type (SyntaxKind (Bit addrSize))) :=
+      match r2e with
+      | nil => None
+      | e :: r2e' =>
+        if (eqb (e (Fin.FS (Fin.FS (Fin.FS (Fin.FS (Fin.FS Fin.F1)))))) exeEpoch)
+        then Some (e Fin.F1)
+        else getArchPcR2E exeEpoch r2e'
+      end.
+
+    Local Definition otake {A} (oa: option A) (default: A): A :=
+      match oa with
+      | Some a => a
+      | None => default
+      end.
+    Infix ">>=" := otake (at level 0, right associativity).
+
+    Definition getArchPc (pcv: fullType type (SyntaxKind (Bit addrSize)))
+               (decEpoch exeEpoch: fullType type (SyntaxKind Bool))
+               (f2i: fullType type (@NativeKind (list (type (Struct F2I))) nil))
+               (i2d: fullType type (@NativeKind (list (type (Struct I2D))) nil))
+               (d2r: fullType type (@NativeKind (list (type (Struct D2R))) nil))
+               (r2e: fullType type (@NativeKind (list (type (Struct R2E))) nil)) :=
+      (getArchPcR2E exeEpoch r2e)
+        >>= (getArchPcD2R exeEpoch d2r)
+        >>= (getArchPcI2D decEpoch exeEpoch i2d)
+        >>= (getArchPcF2I decEpoch exeEpoch f2i)
+        >>= pcv.
+
+    Definition f2iFilter (decEpoch exeEpoch: bool)
+               (f2i: list (type (Struct F2I)))
+      : fullType type (@NativeKind (list (type (Struct F2I))) nil) :=
+      filter
+        (fun e : type (Struct F2I) =>
+           eqb (e Fin.F1 (Fin.FS (Fin.FS Fin.F1))) decEpoch &&
+               eqb (e Fin.F1 (Fin.FS (Fin.FS (Fin.FS Fin.F1)))) exeEpoch) f2i.
+
+    Definition i2dFilter (decEpoch exeEpoch: bool)
+               (i2d: list (type (Struct I2D)))
+      : fullType type (@NativeKind (list (type (Struct I2D))) nil) :=
+      filter
+        (fun e : type (Struct I2D) =>
+           eqb (e Fin.F1 (Fin.FS (Fin.FS Fin.F1))) decEpoch &&
+               eqb (e Fin.F1 (Fin.FS (Fin.FS (Fin.FS Fin.F1)))) exeEpoch) i2d.
+
+    Definition d2rFilter (exeEpoch: bool)
+               (d2r: list (type (Struct D2R)))
+      : fullType type (@NativeKind (list (type (Struct D2R))) nil) :=
+      filter
+        (fun e : type (Struct D2R) =>
+           eqb (e (Fin.FS (Fin.FS (Fin.FS Fin.F1)))) exeEpoch) d2r.
+
+    Definition r2eFilter (exeEpoch: bool)
+               (r2e: list (type (Struct R2E)))
+      : fullType type (@NativeKind (list (type (Struct R2E))) nil) :=
+      filter
+        (fun e : type (Struct R2E) =>
+           eqb (e (Fin.FS (Fin.FS (Fin.FS (Fin.FS (Fin.FS Fin.F1)))))) exeEpoch) r2e.
+
+    Local Definition thetaR (ir sr: RegsT): Prop.
+    Proof.
+      kexistnv "pc" pcv ir (SyntaxKind (Bit addrSize)).
+      kexistnv "decEpoch" decEpochv ir (SyntaxKind Bool).
+      kexistnv "exeEpoch" exeEpochv ir (SyntaxKind Bool).
+      kexistnv "f2i" -- "elt" f2iv ir (@NativeKind (list (type (Struct F2I))) nil).
+      kexistnv "i2d" -- "elt" i2dv ir (@NativeKind (list (type (Struct I2D))) nil).
+      kexistnv "d2r" -- "elt" d2rv ir (@NativeKind (list (type (Struct D2R))) nil).
+      kexistnv "r2e" -- "elt" r2ev ir (@NativeKind (list (type (Struct R2E))) nil).
+
+      exact (sr =
+             ["pc" <- existT _ _ pcv]
+             +["f2i" -- "elt" <- existT _ _ (f2iFilter decEpochv exeEpochv f2iv)]
+             +["i2d" -- "elt" <- existT _ _ (i2dFilter decEpochv exeEpochv i2dv)]
+             +["d2r" -- "elt" <- existT _ _ (d2rFilter exeEpochv d2rv)]
+             +["r2e" -- "elt" <- existT _ _ (r2eFilter exeEpochv r2ev)]
+             +["archPc" <- existT _ _ (getArchPc pcv decEpochv exeEpochv
+                                                 f2iv i2dv d2rv r2ev)])%fmap.
+    Defined.
+
+    Hint Unfold F2I I2D D2R R2E : MethDefs.
+    Hint Unfold getArchPcF2I getArchPcI2D getArchPcD2R getArchPcR2E otake getArchPc
+         f2iFilter i2dFilter d2rFilter r2eFilter thetaR : MapDefs.
+
+    (* TODO *)
+    Local Definition ruleMap (o: RegsT) (n: string) := Some n.
+    Hint Unfold ruleMap : MethDefs.
+
+    Theorem fidreComb_fidreNR: fidreComb <<== fidreNR.
+    Proof.
+      (* apply stepRefinementR with (ruleMap:= ruleMap) (thetaR:= thetaR). *)
+
+      (* - kdecompose_regrel_init. *)
+      (*   meqReify. *)
+
+      (* - intros. *)
+    Admitted.
+
+  End RefinementNR.
+  
+End Processor.
+
